<?xml version='1.0' encoding='utf-8'?>

<section xml:id="DF7" xmlns:xi="http://www.w3.org/2001/XInclude">
  <title>Differentiating implicitly defined functions (DF7)</title>
  <objectives>
    <ul>
      <li>
        <xi:include href="outcomes/07.ptx" />
      </li>
    </ul>
  </objectives>
    <observation>
    Many of the equations that has been discussed so far fall under the category of an explicit equation.  An explicit equation is one in which the relationship between <m>x</m> and <m>y</m> is given explicitly, such as <m>y = f(x)</m>.  In this section we will examine when the relationship between <m>x</m> and <m>y</m> is given implicity. An implicity expression is when the relationship has some equation like <m>f(x,y) = g(x,y)</m> where both sides may depend on both <m>x</m> and <m>y</m>.
    </observation>
    
    <observation>
    Note that if we are taking the derivative with respect to <m>x</m>, then  
        <me>\frac{d}{dx}(f(x)) = f'(x).</me>
        However,
          <me>\frac{d}{dx}(g(y)) = g'(y)\frac{dy}{dx}.</me>
        
    </observation>
  <activity xml:id="activity-derivative-implicit1">
    <introduction>
      <p>
        For this activity we want to find the equation of a tangent line for a circle with radius 5 centered at the origin, <m>x^2+y^2 = 25,</m> at the point <m>(-3,-4).</m>
      </p>
    </introduction>
      <task>
      <statement>
          <p>The derivative with respect to <m>x</m> for the equation of the circle is given by which expression.</p>
          <ol label="A">
                <li><p><m>2x + 2y\frac{dy}{dx} = 25</m></p></li>
                <li><p><m>2x + y\frac{dy}{dx} = 0</m></p></li>
                <li><p><m>2x + 2y\frac{dy}{dx} = 0</m></p></li>
                <li><p><m>2x + 2\frac{dy}{dx} = 25</m></p></li>
            </ol>
          </statement>
      </task>
      <task>
      <statement>
          <p>Solving for <m>\frac{dy}{dx} gives?</m></p>
          <ol label="A">
                <li><p><m>\frac{dy}{dx} = \frac{25-2x}{2y}</m></p></li>
                <li><p><m>\frac{dy}{dx} = -\frac{2x}{y}</m></p></li>
                <li><p><m>\frac{dy}{dx} = -\fraC{x}{y}</m></p></li>
                <li><p><m>\frac{dy}{dx} = \frac{25-2x}{2}</m></p></li>
            </ol>
          </statement>
      </task>
      <task>
      <statement> <p>Plug the point <m>(-3,-4)</m> into the expression found above for the derivative to get the slope of the tangent line.</p>
          </statement>
      </task>
      <task>
      <statement>
          <p>Use the value for the slope of the tangent line to obtaine the equation of the tangent line.</p>
          </statement>
      </task>
  </activity>

    <activity xml:id="activity-derivative-implicit2">
    <introduction>
        <p>The curve given in <xref ref = "figure-derivative-implicit2"/> is an example of an astroid.  The equation of this astoid is <m>x^{2/3} + y^{2/3} = 3^{2/3}</m>.  What is the derivative with respect <m>x</m> for this astroid? (Solve for <m>\frac{dy}{dx}</m>).</p>
        </introduction>
         <figure xml:id="figure-derivative-implicit2">
       <image width="50%" source="derivative_implicit2_graph.png" />
                <caption>Graph of <m>x^{2/3} + y^{2/3} = 3^{2/3}</m>.</caption>
        </figure>
         <ol label="A">
                <li><p><m>\frac{dy}{dx} = \frac{x^{-1/3}}{y^{-1/3}}</m></p></li>
                <li><p><m>\frac{dy}{dx} = \frac{y^{-1/3}}{x^{-1/3}}</m></p></li>
                <li><p><m>\frac{dy}{dx} = \frac{3^{-1/3}-x^{-1/3}}{y^{-1/3}}</m></p></li>
                <li><p><m>\frac{dy}{dx} = -\frac{x^{-1/3}}{y^{-1/3}}</m></p></li>
            </ol>
    </activity>
    
    <activity xml:id="activity-derivative-implicit3">
    <introduction>
        <p>An example of a lemniscate is given in <xref ref = "figure-derivative-implicit3"/>.  The equation of this lemniscate is <m>(x^{2} + y^{2})^2 = x^2 - y^2</m>.  What is the derivative with respect <m>x</m> for this lemniscate? (Solve for <m>\frac{dy}{dx}</m>).</p>
        </introduction>
         <figure xml:id="figure-derivative-implicit3">
       <image width="50%" source="derivative_implicit3_graph.png" />
                <caption>Graph of <m>(x^{2} + y^{2})^2 = x^2 - y^2</m>.</caption>
        </figure>
         <ol label="A">
                <li><p><m>\frac{dy}{dx} = \frac{x(1-2(x^2+y^2))}{y+2(x^2+y^2)}</m></p></li>
                <li><p><m>\frac{dy}{dx} = \frac{x(1-2(x^2+y^2))}{y(1+2(x^2+y^2))}</m></p></li>
                <li><p><m>\frac{dy}{dx} = \frac{y(1+2(x^2+y^2))}{x(1-2(x^2+y^2))}</m></p></li>
                <li><p><m>\frac{dy}{dx} = \frac{y+2(x^2+y^2)}{x(1-2(x^2+y^2))}</m></p></li>
            </ol>
    </activity>
    
</section>