<?xml version='1.0' encoding='utf-8'?>

<section xml:id="IN3" xmlns:xi="http://www.w3.org/2001/XInclude">
  <title>Elementary antiderivatives (IN3)</title>
  <objectives>
    <ul>
      <li>
        <xi:include href="outcomes/03.ptx" />
      </li>
    </ul>
  </objectives>




    <p permid="Kqf">
      In <xref ref="integration-riemann-1"/>, we established that whenever <m>v</m> is constant on an interval,
      the exact distance traveled is the area under the velocity curve.
      When <m>v</m> is not constant,
      we can estimate the total distance traveled by finding the areas of rectangles that approximate the area under the velocity curve.
    </p>

    <p permid="qxo">
      Thus, we see that finding the area between a curve and the horizontal axis is an important exercise:
      besides being an interesting geometric question,
      if the curve gives the velocity of a moving object,
      the area under the curve tells us the exact distance traveled on an interval.
      We can estimate this area if we have a graph or a table of values for the velocity function.
    </p>

    <p permid="WEx">
      In <xref ref="act-4-1-1"/>,
      we encountered an alternate approach to finding the distance traveled.
      If <m>y = v(t)</m> is a formula for the instantaneous velocity
      of a moving object,
      then <m>v</m> must be the derivative of the object's position function,
      <m>s</m>.
      If we can find a formula for <m>s(t)</m> from the formula for <m>v(t)</m>,
      we will know the position of the object at time <m>t</m>,
      and the change in position over a particular time interval tells us the distance traveled on that interval.
    </p>

    <p permid="CLG">
      For example, let's 
      consider the situation from <xref ref="integration-riemann-1"/>,
      where a person is walking along a straight line with velocity function <m>v(t) = 3</m> mph.
    </p>

    <figure xml:id="F-4-1-PA1Soln" permid="Hvz">
      <caption>The velocity function <m>v(t) = 3</m> and corresponding position function <m>s(t) = 3t</m>.</caption>
      <image width="100%" source="4_1_PA1Soln.svg" />
    </figure>

    <p permid="iSP">
      On the left-hand graph of the velocity function in <xref ref="F-4-1-PA1Soln">Figure</xref>,
      we see the relationship between area and distance traveled,
      <me permid="aiX">
        A= 3 \, \frac{\text{miles} }{\text{hour} } \cdot 1.25 \, \text{hours}  = 3.75 \, \text{miles}
      </me>.
      In addition, we observe<fn>
      Here we are making the implicit assumption that <m>s(0) = 0</m>.
      </fn> that if <m>s(t) = 3t</m>,
      then <m>s'(t) = 3</m>, 
      so <m>s(t) = 3t</m> is the position function whose derivative is the given velocity function,
      <m>v(t) = 3</m>.
      The respective locations of the person at times
      <m>t = 0.25</m> and <m>t = 1.5</m> are
      <m>s(1.5) = 4.5</m> and <m>s(0.25) = 0.75</m>, and therefore
      <me permid="Gqg">
        s(1.5) - s(0.25) = 4.5 - 0.75 = 3.75 \ \text{miles}
      </me>.
    </p>

    <p permid="OZY">
      This is the person's change in position on <m>[0.25,1.5]</m>,
      which is precisely the distance traveled.
      
    </p>

    <p permid="vhh">
     Observe that if we know a formula for a velocity function <m>v</m>,
      it can be very helpful to find a function <m>s</m> that satisfies <m>s' = v</m>.
      We say that <m>s</m> is an
      <em>antiderivative</em> of <m>v</m>.
      More generally, we have the following formal definition.
    </p>

          
    <!--DEFINITION OF ANTIDERIVATIVE from Active Calculus -->
    <definition permid="dzc">
      <statement>
        <p permid="ctJ">
          If <m>g</m> and <m>G</m> are functions such that <m>G' = g</m>,
          we say that <m>G</m> is an <term>antiderivative</term>
              <idx><h>antiderivative</h></idx>
          of <m>g</m>.
        </p>
      </statement>
    </definition>

    <p permid="boq">
      For example, if <m>g(x) = 3x^2 + 2x</m>,
      <m>G(x) = x^3 + x^2</m> is an antiderivative of <m>g</m>,
      because <m>G'(x) = g(x)</m>.
      Note that we say <q>an</q>
      antiderivative of <m>g</m> rather than <q>the</q>
      antiderivative of <m>g</m>, because
      <m>H(x) = x^3 + x^2 + 5</m> is also a function whose derivative is <m>g</m>,
      and thus <m>H</m> is another antiderivative of <m>g</m>.
    </p>

<!-- FROM 4-4-2 IN ACTIVE CALCULUS -->

    <p permid="PRj">
      The general problem of finding an antiderivative is difficult.
      In part, this is due to the fact that we are trying to undo the process of differentiating,
      and the undoing is much more difficult than the doing. However, some antiderivatives can be fairly simple to find if we remember our elementary derivative rules. (See <xref ref="DF3"/>.)</p>
      
     <activity xml:id="elem-antider-intro">
        <statement>
    <p>Consider the function <m>f(x)=\cos x</m>. Which of the following could be <m>F(x)</m>, an antiderivative of <m>f(x)</m>? </p>
    <ol label="A">
                <li><p> <m>\sin x</m> </p></li>
                <li><p> <m>\cos x</m> </p></li>
                <li><p> <m>\tan x</m> </p></li>
                <li><p> <m>\sec x</m> </p></li>

            </ol>
    </statement>
        </activity>   
    
        
             <activity xml:id="elem-antider-intro2">
        <statement>
    <p>Consider the function <m>f(x)=x^2</m>. Which of the following could be <m>F(x)</m>, an antiderivative of <m>f(x)</m>? </p>
    <ol label="A">
               <li><p><m> 2x </m></p></li>
               <li><p><m> \frac{1}{3}x^3 </m></p></li>
               <li><p><m> x^3</m></p></li>
               <li><p><m> \frac{2}{3}x^3 </m></p></li>

            </ol>
    </statement>
        </activity>   
       
<!--         
        
        For example,
      while it is evident that an antiderivative of <m>f(x) = \sin(x)</m> is
      <m>F(x) = -\cos(x)</m> and that an antiderivative of
      <m>g(x) = x^2</m> is <m>G(x) = \frac{1}{3} x^3</m>,
      combinations of <m>f</m> and <m>g</m> can be far more complicated.
      Consider the functions
      <me permid="rYt">
        5\sin(x) - 4x^2, \ x^2 \sin(x), \ \frac{\sin(x)}{x^2}, \ \text{and}  \ \sin(x^2)
      </me>.
    </p>

    <p permid="vYs">
      What is involved in trying to find an antiderivative for each?
      From our experience with derivative rules,
      we know that derivatives of sums and constant multiples of basic functions are simple to execute, but
      derivatives involving products, quotients,
      and composites of familiar functions are more complicated.
      Therefore, it stands to reason that antidifferentiating products,
      quotients,
      and composites of basic functions may be even more challenging.
      We defer our study of all but the most elementary antiderivatives to later in the text.
    </p> -->

    <p permid="cfB">
      We now note that whenever we know the derivative of a function,
      we have a <em>function-derivative pair</em>,
      so we also know the antiderivative of a function.
      For instance, in <xref ref="elem-antider-intro"/> we could use our prior knowledge that 
      <me permid="YfC">
        \frac{d}{dx}[\sin(x)] = \cos(x)
      </me>,
     to determine that <m>F(x) = \sin(x)</m> is an antiderivative of <m>f(x) = \cos(x)</m>.
      <m>F</m> and <m>f</m> together form a function-derivative pair.
      Every elementary derivative rule leads us to such a pair,
      and thus to a known antiderivative.
    </p>

<!-- FINISH EDITING FROM HERE!!!!!!!!!!!!!!!!!!!!!!!!!!!!!!!!!!!!!!!!!!!!!!!!!!!!!!!!!!!!!!!!!!!!!!!!!!!!!!!!!!!!!!!!!!!!!!!!!!!!!!!!!!!!!  -->

    <p permid="otT">
      Finally, before proceeding to build a list of common functions whose antiderivatives we know,
      we recall that each function has more than one antiderivative.
      Because the derivative of any constant is zero,
      we may add a constant of our choice to 
      any antiderivative.
      For instance, we know that
      <m>G(x) = \frac{1}{3}x^3</m> is an antiderivative of <m>g(x) = x^2</m>.
      But we could also have chosen <m>G(x) = \frac{1}{3}x^3 + 7</m>,
      since in this case as well, <m>G'(x) = x^2</m>.

      If <m>g(x) = x^2</m>, we say that the
      <em>general antiderivative</em>
          <idx><h>antiderivative</h><h>general</h></idx>
      of <m>g</m> is
      <me permid="ktU">
        G(x) = \frac{1}{3}x^3 + C
      </me>,
      where <m>C</m> represents an arbitrary real number constant.
      Regardless of the formula for <m>g</m>,
      including <m>+C</m> in the formula for its antiderivative <m>G</m> results in the most general possible antiderivative.
    </p>

    <p permid="UBc">
      Our current interest in antiderivatives is so that we can evaluate definite integrals 
      by the Fundamental Theorem of Calculus.
      For that task, the constant <m>C</m> is irrelevant,
      and we usually omit it.
      To see why, consider the definite integral
      <me permid="QBd">
        \int_0^1 x^2 \, dx
      </me>.
    </p>

    <p permid="AIl">
      For the integrand <m>g(x) = x^2</m>,
      suppose we find and use the general antiderivative <m>G(x) = \frac{1}{3} x^3 + C</m>.
      Then, by the FTC,
      <md permid="wIm">
        <mrow>\int_0^1 x^2 \, dx &amp;=  \left. \frac{1}{3} x^3 + C \right|_0^1</mrow>
        <mrow>&amp;= \left(\frac{1}{3} (1)^3 + C  \right) - \left(\frac{1}{3} (0)^3 + C  \right)</mrow>
        <mrow>&amp;= \frac{1}{3} + C - 0 - C</mrow>
        <mrow>&amp;= \frac{1}{3}</mrow>
      </md>.
    </p>

    <p permid="gPu">
      Observe that the <m>C</m>-values appear as opposites in the evaluation of the integral and thus do not affect the definite integral's value.
    </p>

    <p permid="MWD">
      In the following activity,
      we work to build a list of basic functions whose antiderivatives we already know.
    </p>

<activity xmlns:xi="http://www.w3.org/2001/XInclude" xml:id="act-4-4-2" permid="ovP">
  <statement>
    <p permid="yUU">
      Use your knowledge of derivatives of basic functions to complete <xref ref="T-4-4-Act2">Table</xref> of antiderivatives.
      For each entry,
      your task is to find a function <m>F</m> whose derivative is the given function <m>f</m>.
      When finished,
      use the FTC and the results in the table to evaluate the three given definite integrals.
    </p>

    <table xml:id="T-4-4-Act2" permid="PTf">
      <caption>Familiar basic functions and their antiderivatives.</caption>
      <tabular top="minor" bottom="minor" permid="wao">
        <row bottom="medium">
          <cell>given function, <m>f(x)</m></cell>
          <cell>antiderivative, <m>F(x)</m>   <nbsp /></cell>
        </row>
        <row>
          <cell  ><m>k</m>, (<m>k</m> is constant)</cell>
          <cell></cell>
        </row>
        <row>
          <cell><m>x^n</m>, <m>n \ne -1</m></cell>
          <cell></cell>
        </row>
        <row>
          <cell><m>\frac{1}{x}</m>, <m>x \gt 0</m></cell>
          <cell></cell>
        </row>
        <row>
          <cell><m>\sin(x)</m></cell>
          <cell></cell>
        </row>
        <row>
          <cell><m>\cos(x)</m></cell>
          <cell></cell>
        </row>
        <row>
          <cell><m>\sec(x) \tan(x)</m></cell>
          <cell></cell>
        </row>
        <row>
          <cell><m>\csc(x) \cot(x)</m></cell>
          <cell></cell>
        </row>
        <row>
          <cell><m>\sec^2 (x)</m></cell>
          <cell></cell>
        </row>
        <row>
          <cell><m>\csc^2 (x)</m></cell>
          <cell></cell>
        </row>
        <row>
          <cell><m>e^x</m></cell>
          <cell></cell>
        </row>
        <row>
          <cell><m>a^x</m> <m>(a \gt 1)</m></cell>
          <cell></cell>
        </row>
        <row>
          <cell><m>\frac{1}{1+x^2}</m></cell>
          <cell></cell>
        </row>
        <row>
          <cell><m>\frac{1}{\sqrt{1-x^2}}</m></cell>
          <cell></cell>
        </row>
      </tabular>

    </table>

  
  </statement>
<!--   <hint permid="bxD">
    <p permid="SNL">
      For the table,
      you might start by constructing a list of all the basic functions whose derivative you know.
      For the three definite integrals,
      be sure to recall the sum and constant multiple rules,
      which work not only for differentiating,
      but also for antidifferentiating.
    </p>
  </hint>
  <answer permid="vqu">
    <sidebyside permid="chx">

      <tabular top="minor" bottom="minor" permid="jLW">
        <row bottom="medium">
          <cell>given function, <m>f(x)</m></cell>
          <cell>antiderivative, <m>F(x)</m>   <nbsp /></cell>
        </row>
        <row>
          <cell  ><m>k</m>, (<m>k \ne 0</m>)</cell>
          <cell><m>kx</m></cell>
        </row>
        <row>
          <cell><m>x^n</m>, <m>n \ne -1</m></cell>
          <cell><m>\frac{1}{n+1}x^{n+1}</m></cell>
        </row>
        <row>
          <cell><m>\frac{1}{x}</m>, <m>x \gt 0</m></cell>
          <cell><m>\ln(x)</m></cell>
        </row>
        <row>
          <cell><m>\sin(x)</m></cell>
          <cell><m>-\cos(x)</m></cell>
        </row>
        <row>
          <cell><m>\cos(x)</m></cell>
          <cell><m>\sin(x)</m></cell>
        </row>
        <row>
          <cell><m>\sec(x) \tan(x)</m></cell>
          <cell><m>\sec(x)</m></cell>
        </row>
        <row>
          <cell><m>\csc(x) \cot(x)</m></cell>
          <cell><m>-\csc(x)</m></cell>
        </row>
        <row>
          <cell><m>\sec^2 (x)</m></cell>
          <cell><m>\tan(x)</m></cell>
        </row>
        <row>
          <cell><m>\csc^2 (x)</m></cell>
          <cell><m>-\cot(x)</m></cell>
        </row>
        <row>
          <cell><m>e^x</m></cell>
          <cell><m>e^x</m></cell>
        </row>
        <row>
          <cell><m>a^x</m> <m>(a \gt 1)</m></cell>
          <cell><m>\frac{1}{\ln(a)} a^x</m></cell>
        </row>
        <row>
          <cell><m>\frac{1}{1+x^2}</m></cell>
          <cell><m>\arctan(x)</m></cell>
        </row>
        <row>
          <cell><m>\frac{1}{\sqrt{1-x^2}}</m></cell>
          <cell><m>\arcsin(x)</m></cell>
        </row>
      </tabular>

    </sidebyside>

    <p permid="mGC">
      <ol label="a." permid="nLV">
        <li permid="svO">
          <p permid="VIr">
            <m> \int_0^1 \left(x^3 - x - e^x + 2\right) \,dx = \frac{11}{4} - e</m>.
          </p>
        </li>

        <li permid="YCX">
          <p permid="BPA">
            <m> \int_0^{\pi/3} (2\sin (t) - 4\cos(t) + \sec^2(t) - \pi) \, dt = 1 - \sqrt{3} - \frac{\pi^2}{3}</m>.
          </p>
        </li>

        <li permid="EKg">
          <p permid="hWJ">
            <m> \int_0^1 (\sqrt{x} - x^2) \, dx = \frac{1}{3}</m>.
          </p>
        </li>
      </ol>
    </p>
  </answer>
  <solution permid="Pjl">
    <sidebyside permid="IoG">

      <tabular top="minor" bottom="minor" permid="DEN">
        <row bottom="medium">
          <cell>given function, <m>f(x)</m></cell>
          <cell>antiderivative, <m>F(x)</m>   <nbsp /></cell>
        </row>
        <row>
          <cell  ><m>k</m>, (<m>k \ne 0</m>)</cell>
          <cell><m>kx</m></cell>
        </row>
        <row>
          <cell><m>x^n</m>, <m>n \ne -1</m></cell>
          <cell><m>\frac{1}{n+1}x^{n+1}</m></cell>
        </row>
        <row>
          <cell><m>\frac{1}{x}</m>, <m>x \gt 0</m></cell>
          <cell><m>\ln(x)</m></cell>
        </row>
        <row>
          <cell><m>\sin(x)</m></cell>
          <cell><m>-\cos(x)</m></cell>
        </row>
        <row>
          <cell><m>\cos(x)</m></cell>
          <cell><m>\sin(x)</m></cell>
        </row>
        <row>
          <cell><m>\sec(x) \tan(x)</m></cell>
          <cell><m>\sec(x)</m></cell>
        </row>
        <row>
          <cell><m>\csc(x) \cot(x)</m></cell>
          <cell><m>-\csc(x)</m></cell>
        </row>
        <row>
          <cell><m>\sec^2 (x)</m></cell>
          <cell><m>\tan(x)</m></cell>
        </row>
        <row>
          <cell><m>\csc^2 (x)</m></cell>
          <cell><m>-\cot(x)</m></cell>
        </row>
        <row>
          <cell><m>e^x</m></cell>
          <cell><m>e^x</m></cell>
        </row>
        <row>
          <cell><m>a^x</m> <m>(a \gt 1)</m></cell>
          <cell><m>\frac{1}{\ln(a)} a^x</m></cell>
        </row>
        <row>
          <cell><m>\frac{1}{1+x^2}</m></cell>
          <cell><m>\arctan(x)</m></cell>
        </row>
        <row>
          <cell><m>\frac{1}{\sqrt{1-x^2}}</m></cell>
          <cell><m>\arcsin(x)</m></cell>
        </row>
      </tabular>

    </sidebyside>

    <p permid="Gzt">
      <ol label="a." permid="HEM">
        <li permid="kRp">
          <p permid="OdS">
            By standard antiderivative rules and the FTC,
            <md permid="Ljm">
              <mrow>\int_0^1 \left(x^3 - x - e^x + 2\right) \,dx =\mathstrut \amp  \left. \frac{1}{4} x^4 - \frac{1}{2}x^2 - e^x + 2x \right|_0^1</mrow>
              <mrow>=\mathstrut \amp  \left(\frac{1}{4} (1)^4 - \frac{1}{2}(1)^2 - e^1 + 2(1) \right) -   \left(\frac{1}{4} (0)^4 - \frac{1}{2}(0)^2 - e^0 + 2(0) \right)</mrow>
              <mrow>=\mathstrut \amp  \frac{1}{4} - \frac{1}{2} - e + 2 -  \left(0 - 0 - 1 + 0 \right)</mrow>
              <mrow>=\mathstrut \amp  -\frac{1}{4} - e + 3</mrow>
              <mrow>=\mathstrut \amp  \frac{11}{4} - e</mrow>
            </md>.
          </p>
        </li>

        <li permid="QYy">
          <p permid="ulb">
            Calculating the needed antiderivative and applying the FTC,
            <md permid="rqv">
              <mrow>\int_0^{\pi/3} (2\sin (t) - 4\cos(t) + \sec^2(t) - \pi) \, dt =\mathstrut \amp  \left. \left(-2\cos(t) - 4\sin(t) + \tan(t) - \pi t \right) \right|_0^{\pi/3}</mrow>
              <mrow>=\mathstrut \amp  \left(-2\cos(\pi/3) - 4\sin(\pi/3) + \tan(\pi/3) - \pi (\pi/3) \right) -</mrow>
              <mrow>\ \amp   \left(-2\cos(0)) - 4\sin(0) + \tan(0) - \pi (0) \right)</mrow>
              <mrow>=\mathstrut \amp  -2 \cdot \frac{1}{2} - 4 \cdot \frac{\sqrt{3}}{2} + \sqrt{3} - \frac{\pi^2}{3} - (-2 - 0 + 0 - 0)</mrow>
              <mrow>=\mathstrut \amp  1 - \sqrt{3} - \frac{\pi^2}{3}</mrow>
            </md>.
          </p>
        </li>

        <li permid="xfH">
          <p permid="ask">
            Noting that <m>\frac{d}{dx}[\frac{2}{3} x^{3/2}] = x^{1/2}</m>,
            we find that
            <md permid="XxE">
              <mrow>\int_0^1 (\sqrt{x} - x^2) \, dx =\mathstrut \amp  \left. \frac{2}{3}x^{3/2} - \frac{1}{3}x^3 \right|_0^1</mrow>
              <mrow>=\mathstrut \amp  \frac{2}{3} - \frac{1}{3} - (0 - 0 )</mrow>
              <mrow>=\mathstrut \amp  \frac{1}{3}</mrow>
            </md>.
          </p>
        </li>
      </ol>
    </p>
  </solution> -->
</activity>


   <p permid="ImK">
      In <xref ref="act-4-4-2">Activity</xref>,
      we constructed a list of the basic antiderivatives we know at this time.
      Those rules will help us  antidifferentiate sums and constant multiples of basic functions.
      For example,
      since <m>-\cos(x)</m> is an antiderivative of <m>\sin(x)</m> and
      <m>\frac{1}{3}x^3</m> is an antiderivative of <m>x^2</m>,
      it follows that
      <me permid="EmL">
        F(x) = -5\cos(x) - \frac{4}{3}x^3
      </me>
      is an antiderivative of <m>f(x) = 5\sin(x) - 4x^2</m>,
      by the sum and constant multiple rules for differentiation.
    </p>    
 
<!-- indefinite integral notation         -->
        
     <p permid="Ojn">
      It is useful to have shorthand notation that indicates the instruction to find an antiderivative.
      Thus, in a similar way to how the notation
      <me permid="RNN">
        \frac{d}{dx} \left[ f(x) \right]
      </me>
      represents the derivative of <m>f(x)</m> with respect to <m>x</m>,
      we use the notation of the <em>indefinite integral</em>,
          <idx><h>indefinite integral</h></idx>
      <me permid="xUW">
        \int f(x) \, dx
      </me>
      to represent the general antiderivative of <m>f</m> with respect to <m>x</m>.
      Returning to the earlier example with <m>h(x) = (5x-3)^6</m>,
      we can rephrase the relationship between <m>h</m> and its antiderivative <m>H</m> through the notation
      <me permid="ecf">
        \int (5x-3)^6 \, dx = \frac{1}{35} (5x-6)^7 + C
      </me>.
    </p>

    <p permid="uqw">
      When we find an antiderivative,
      we will often say that we <em>evaluate an indefinite integral</em>.
          <idx><h>indefinite integral</h><h>evaluate</h></idx>
      Just as the notation <m>\frac{d}{dx} [ \Box ]</m> means
      <q>find the derivative with respect to <m>x</m> of <m>\Box</m>,</q>
      the notation <m>\int \Box \, dx</m> means
      <q>find a function of <m>x</m> whose derivative is <m>\Box</m>.</q>
    </p> 
    
</section>














